Added chapters and sections to Ticket Lock. Restructured chapter. Created auxiliary predicate locked_by. Refactored invariant to use previously defined predicates. Added guiding comments. Rephrasing and formatting.

exercises/ticket_lock.v
@@ -2,25 +2,43 @@ From iris.algebra Require Import auth excl gset numbers.
 From iris.base_logic.lib Require Export invariants.
 From iris.heap_lang Require Import lang proofmode notation.
 
+(* ################################################################# *)
+(** * Case Study: Ticket Lock *)
+
+(* ================================================================= *)
+(** ** Implementation *)
+
 (**
-  Let's look at another implementation of a lock, namely a ticket
-  lock. Instead of having every thread fight to acquire the lock. The
-  ticket lock makes them wait in line. It does this by maintaining two
-  counters representing queue positions. The first counter is the
-  position next in line to access the critical region. While the
-  second counter is the end of the line.
-  A thread can acquire the lock by incrementing the second counter and
-  keeping its previous value as a ticket for its position in the
-  queue. When the first counter reaches this ticket value, the thread
-  gains access to the critical region. The thread can then release the
-  lock by incrementing the first counter.
+  Let us look at another implementation of a lock, namely a ticket lock.
+  Instead of having every thread fight to acquire the lock, the ticket
+  lock makes them wait in line. It functions similarly to a ticketing
+  system that one often finds in bakeries and pharmacies. Upon entering
+  the shop, you pick a ticket with some number and wait until the number
+  on the screen has reached your number. Once this happen, it becomes
+  your turn to speak to the shop assistant. In our scenario, talking to
+  the shop assistant corresponds to accessing the protected resources.
+
+  To implement this, we will maintain two counters: [o] and [n]. The
+  first counter, [o], represent the number on the screen – the customer
+  currently being served. The second counter, [n], represents the next
+  number to be dispensed by the ticketing machine.
+
+  To acquire the lock, a thread must increment the second counter, [n],
+  and keep its previous value as a ticket for a position in the queue.
+  Once the ticket has been obtained, the thread must wait until the
+  first counter, [o], reaches its ticket value. Once this happens, the
+  thread gets access the protected resources. The thread can then
+  release the lock by incrementing the first counter.
 *)
+
 Definition mk_lock : val :=
   λ: <>, (ref #0, ref #0).
+
 Definition wait : val :=
   rec: "wait" "n" "l" :=
   let: "o" := !(Fst "l") in
   if: "o" = "n" then #() else "wait" "n" "l".
+
 Definition acquire : val :=
   rec: "acquire" "l" :=
   let: "n" := !(Snd "l") in
@@ -28,13 +46,19 @@ Definition acquire : val :=
     wait "n" "l"
   else
     "acquire" "l".
+
 Definition release : val :=
   λ: "l", Fst "l" <- ! (Fst "l") + #1.
 
+(* ================================================================= *)
+(** ** Representation Predicates *)
+
 (**
-  As a ticket lock is a lock. So we expect it to satisfy the same
-  specification as the spin lick. This time you have to find the
-  necessary resource and lock invariant by yourself.
+  As a ticket lock is a lock, we expect it to satisfy the same
+  specification as the spin-lock. This time you have to come up with the
+  necessary resource algebra and lock invariant by yourself. It might be
+  instructive to first look through all required predicates and
+  specifications to figure out exactly what needs to be proven.
 *)
 
 Definition RA : cmra
@@ -44,39 +68,62 @@ Section proofs.
 Context `{!heapGS Σ, !inG Σ RA}.
 Let N := nroot .@ "ticket_lock".
 
-Definition lock_inv (γ : gname) (lo ln : loc) (P : iProp Σ) : iProp Σ
+(**
+  This time around, we know that the thread is locked by a thread with a
+  specific ticket. As such, we first define a predicate [locked_by]
+  which states that the lock is locked by ticket [o].
+*)
+Definition locked_by (γ : gname) (o : nat) : iProp Σ
   (* := insert your definition here *). Admitted.
 
-Definition is_lock (γ : gname) (l : val) (P : iProp Σ) : iProp Σ :=
-  ∃ lo ln : loc, ⌜l = (#lo, #ln)%V⌝ ∗ inv N (lock_inv γ lo ln P).
-
-Definition locked (γ : gname) : iProp Σ
-  (* := insert your definition here *). Admitted.
-
-Definition issued (γ : gname) (x : nat) : iProp Σ
-  (* := insert your definition here *). Admitted.
+(** The lock is locked when it has been locked by some ticket. *)
+Definition locked (γ : gname) : iProp Σ :=
+  ∃ o, locked_by γ o.
 
 Lemma locked_excl γ : locked γ -∗ locked γ -∗ False.
 Proof.
   (* exercise *)
 Admitted.
 
-Lemma mk_lock_spec P : {{{ P }}} mk_lock #() {{{ γ l, RET l; is_lock γ l P }}}.
+(**
+  We will also have a predicate signifying that ticket [x] has been
+  _issued_. A thread will need to have been issued ticket [x] in order
+  to wait for the first counter to become [x].
+*)
+Definition issued (γ : gname) (x : nat) : iProp Σ
+  (* := insert your definition here *). Admitted.
+
+Definition lock_inv (γ : gname) (lo ln : loc) (P : iProp Σ) : iProp Σ
+  (* := insert your definition here *). Admitted.
+
+Definition is_lock (γ : gname) (l : val) (P : iProp Σ) : iProp Σ :=
+  ∃ lo ln : loc, ⌜l = (#lo, #ln)%V⌝ ∗ inv N (lock_inv γ lo ln P).
+
+(* ================================================================= *)
+(** ** Specifications *)
+
+Lemma mk_lock_spec P :
+  {{{ P }}} mk_lock #() {{{ γ l, RET l; is_lock γ l P }}}.
 Proof.
   (* exercise *)
 Admitted.
 
-Lemma wait_spec γ l P x : {{{ is_lock γ l P ∗ issued γ x }}} wait #x l {{{ RET #(); locked γ ∗ P }}}.
+Lemma wait_spec γ l P x :
+  {{{ is_lock γ l P ∗ issued γ x }}}
+    wait #x l
+  {{{ RET #(); locked γ ∗ P }}}.
 Proof.
   (* exercise *)
 Admitted.
 
-Lemma acquire_spec γ l P : {{{ is_lock γ l P }}} acquire l {{{ RET #(); locked γ ∗ P }}}.
+Lemma acquire_spec γ l P :
+  {{{ is_lock γ l P }}} acquire l {{{ RET #(); locked γ ∗ P }}}.
 Proof.
   (* exercise *)
 Admitted.
 
-Lemma release_spec γ l P : {{{ is_lock γ l P ∗ locked γ ∗ P }}} release l {{{ RET #(); True }}}.
+Lemma release_spec γ l P :
+  {{{ is_lock γ l P ∗ locked γ ∗ P }}} release l {{{ RET #(); True }}}.
 Proof.
   (* exercise *)
 Admitted.
