theories/ticket_lock.v
@@ -2,25 +2,43 @@ From iris.algebra Require Import auth excl gset numbers.
 From iris.base_logic.lib Require Export invariants.
 From iris.heap_lang Require Import lang proofmode notation.
 
+(* ################################################################# *)
+(** * Case Study: Ticket Lock *)
+
+(* ================================================================= *)
+(** ** Implementation *)
+
 (**
-  Let's look at another implementation of a lock, namely a ticket
-  lock. Instead of having every thread fight to acquire the lock. The
-  ticket lock makes them wait in line. It does this by maintaining two
-  counters representing queue positions. The first counter is the
-  position next in line to access the critical region. While the
-  second counter is the end of the line.
-  A thread can acquire the lock by incrementing the second counter and
-  keeping its previous value as a ticket for its position in the
-  queue. When the first counter reaches this ticket value, the thread
-  gains access to the critical region. The thread can then release the
-  lock by incrementing the first counter.
+  Let us look at another implementation of a lock, namely a ticket lock.
+  Instead of having every thread fight to acquire the lock, the ticket
+  lock makes them wait in line. It functions similarly to a ticketing
+  system that one often finds in bakeries and pharmacies. Upon entering
+  the shop, you pick a ticket with some number and wait until the number
+  on the screen has reached your number. Once this happen, it becomes
+  your turn to speak to the shop assistant. In our scenario, talking to
+  the shop assistant corresponds to accessing the protected resources.
+
+  To implement this, we will maintain two counters: [o] and [n]. The
+  first counter, [o], represent the number on the screen – the customer
+  currently being served. The second counter, [n], represents the next
+  number to be dispensed by the ticketing machine.
+
+  To acquire the lock, a thread must increment the second counter, [n],
+  and keep its previous value as a ticket for a position in the queue.
+  Once the ticket has been obtained, the thread must wait until the
+  first counter, [o], reaches its ticket value. Once this happens, the
+  thread gets access the protected resources. The thread can then
+  release the lock by incrementing the first counter.
 *)
+
 Definition mk_lock : val :=
   λ: <>, (ref #0, ref #0).
+
 Definition wait : val :=
   rec: "wait" "n" "l" :=
   let: "o" := !(Fst "l") in
   if: "o" = "n" then #() else "wait" "n" "l".
+
 Definition acquire : val :=
   rec: "acquire" "l" :=
   let: "n" := !(Snd "l") in
@@ -28,24 +46,35 @@ Definition acquire : val :=
     wait "n" "l"
   else
     "acquire" "l".
+
 Definition release : val :=
   λ: "l", Fst "l" <- ! (Fst "l") + #1.
 
+(* ================================================================= *)
+(** ** Representation Predicates *)
+
 (**
-  As a ticket lock is a lock. So we expect it to satisfy the same
-  specification as the spin lick. This time you have to find the
-  necessary resource and lock invariant by yourself.
+  As a ticket lock is a lock, we expect it to satisfy the same
+  specification as the spin-lock. This time you have to come up with the
+  necessary resource algebra and lock invariant by yourself. It might be
+  instructive to first look through all required predicates and
+  specifications to figure out exactly what needs to be proven.
 *)
 
 Definition RA : cmra
 (* BEGIN SOLUTION *)
   (**
     We will use a finite set of numbers to represent the tickets that
-    have been issued. This becomes a camera by using the disjoint
-    union as an operation.
-    For the first counter, we will use an exclusive camera. By wrapping
-    them both in an authoritative camera, we can use the authoritative
-    fragment to bind the values of our counters to the ghost state.
+    have been issued – the second counter. This becomes a camera by
+    using the disjoint union as an operation.
+
+    For the first counter, we will use the exclusive camera over the
+    natural numbers – this means that there can be only one
+    access-granting ticket owned at a time.
+
+    By wrapping them both in an authoritative camera, we can use the
+    authoritative fragment to bind the values of our counters to the
+    ghost state.
   *)
   := authR (prodUR (optionUR (exclR natO)) (gset_disjR nat)).
 (* END SOLUTION BEGIN TEMPLATE
@@ -56,47 +85,25 @@ Section proofs.
 Context `{!heapGS Σ, !inG Σ RA}.
 Let N := nroot .@ "ticket_lock".
 
-Definition lock_inv (γ : gname) (lo ln : loc) (P : iProp Σ) : iProp Σ
+(**
+  This time around, we know that the thread is locked by a thread with a
+  specific ticket. As such, we first define a predicate [locked_by]
+  which states that the lock is locked by ticket [o].
+*)
+Definition locked_by (γ : gname) (o : nat) : iProp Σ
 (* BEGIN SOLUTION *)
   (**
-    Our invariant will first link the authoritative fragment to the
-    counters. For the second counter, this means that all tickets prior
-    to the counter's current value must have been issued.
-    Secondly the lock either contains the current ticket, or access to
-    the critical area, as well as ownership of the value of the first
-    counter.
+    We know that the lock is locked by ticket [o] when we have ownership
+    of the exclusive counter being [o].
   *)
-  := ∃ o n : nat, lo ↦ #o ∗ ln ↦ #n ∗
-  own γ (● (Excl' o, GSet (set_seq 0 n))) ∗
-  (
-    (own γ (◯ (Excl' o, GSet ∅)) ∗ P) ∨
-    own γ (◯ (ε : option (excl nat), GSet {[o]}))
-  ).
+  := own γ (◯ (Excl' o, GSet ∅)).
 (* END SOLUTION BEGIN TEMPLATE
   (* := insert your definition here *). Admitted.
 END TEMPLATE *)
 
-Definition is_lock (γ : gname) (l : val) (P : iProp Σ) : iProp Σ :=
-  ∃ lo ln : loc, ⌜l = (#lo, #ln)%V⌝ ∗ inv N (lock_inv γ lo ln P).
-
-Definition locked (γ : gname) : iProp Σ
-(* BEGIN SOLUTION *)
-  (**
-    The lock will be locked when the ownership of the first counters
-    value is not in the invariant.
-  *)
-  := ∃ o, own γ (◯ (Excl' o, GSet ∅)).
-(* END SOLUTION BEGIN TEMPLATE
-  (* := insert your definition here *). Admitted.
-END TEMPLATE *)
-
-Definition issued (γ : gname) (x : nat) : iProp Σ
-(* BEGIN SOLUTION *)
-  (** A ticket is simply the singleton set over its index. *)
-  := own γ (◯ (ε : option (excl nat), GSet {[x]})).
-(* END SOLUTION BEGIN TEMPLATE
-  (* := insert your definition here *). Admitted.
-END TEMPLATE *)
+(** The lock is locked when it has been locked by some ticket. *)
+Definition locked (γ : gname) : iProp Σ :=
+  ∃ o, locked_by γ o.
 
 Lemma locked_excl γ : locked γ -∗ locked γ -∗ False.
 (* SOLUTION *) Proof.
@@ -107,7 +114,49 @@ Lemma locked_excl γ : locked γ -∗ locked γ -∗ False.
   by destruct H as [H _].
 Qed.
 
-Lemma mk_lock_spec P : {{{ P }}} mk_lock #() {{{ γ l, RET l; is_lock γ l P }}}.
+(**
+  We will also have a predicate signifying that ticket [x] has been
+  _issued_. A thread will need to have been issued ticket [x] in order
+  to wait for the first counter to become [x].
+*)
+Definition issued (γ : gname) (x : nat) : iProp Σ
+(* BEGIN SOLUTION *)
+  (** A ticket is simply the singleton set over its index. *)
+  := own γ (◯ (ε : option (excl nat), GSet {[x]})).
+(* END SOLUTION BEGIN TEMPLATE
+  (* := insert your definition here *). Admitted.
+END TEMPLATE *)
+
+Definition lock_inv (γ : gname) (lo ln : loc) (P : iProp Σ) : iProp Σ
+(* BEGIN SOLUTION *)
+  (**
+    Our invariant will first link the authoritative fragment to the
+    counters. For the second counter, this means that all tickets prior
+    to the counter's current value must have been issued.
+
+    Secondly, the lock contains either ownership of the value of the
+    first counter as well as the protected resources (the queue is
+    unlocked), or the current access-granting ticket (the queue is
+    locked).
+  *)
+  := ∃ o n : nat, lo ↦ #o ∗ ln ↦ #n ∗
+  own γ (● (Excl' o, GSet (set_seq 0 n))) ∗
+  (
+    (locked_by γ o ∗ P) ∨
+    issued γ o
+  ).
+(* END SOLUTION BEGIN TEMPLATE
+  (* := insert your definition here *). Admitted.
+END TEMPLATE *)
+
+Definition is_lock (γ : gname) (l : val) (P : iProp Σ) : iProp Σ :=
+  ∃ lo ln : loc, ⌜l = (#lo, #ln)%V⌝ ∗ inv N (lock_inv γ lo ln P).
+
+(* ================================================================= *)
+(** ** Specifications *)
+
+Lemma mk_lock_spec P :
+  {{{ P }}} mk_lock #() {{{ γ l, RET l; is_lock γ l P }}}.
 (* SOLUTION *) Proof.
   iIntros "%Φ HP HΦ".
   wp_lam.
@@ -127,7 +176,10 @@ Lemma mk_lock_spec P : {{{ P }}} mk_lock #() {{{ γ l, RET l; is_lock γ l P }}}
   iFrame.
 Qed.
 
-Lemma wait_spec γ l P x : {{{ is_lock γ l P ∗ issued γ x }}} wait #x l {{{ RET #(); locked γ ∗ P }}}.
+Lemma wait_spec γ l P x :
+  {{{ is_lock γ l P ∗ issued γ x }}}
+    wait #x l
+  {{{ RET #(); locked γ ∗ P }}}.
 (* SOLUTION *) Proof.
   iIntros "%Φ [(%lo & %ln & -> & #I) Hx] HΦ".
   iLöb as "IH".
@@ -165,7 +217,8 @@ Lemma wait_spec γ l P x : {{{ is_lock γ l P ∗ issued γ x }}} wait #x l {{{ 
     iApply ("IH" with "Hx HΦ").
 Qed.
 
-Lemma acquire_spec γ l P : {{{ is_lock γ l P }}} acquire l {{{ RET #(); locked γ ∗ P }}}.
+Lemma acquire_spec γ l P :
+  {{{ is_lock γ l P }}} acquire l {{{ RET #(); locked γ ∗ P }}}.
 (* SOLUTION *) Proof.
   iIntros "%Φ (%lo & %ln & -> & #I) HΦ".
   iLöb as "IH".
@@ -215,7 +268,8 @@ Lemma acquire_spec γ l P : {{{ is_lock γ l P }}} acquire l {{{ RET #(); locked
     by iApply "IH".
 Qed.
 
-Lemma release_spec γ l P : {{{ is_lock γ l P ∗ locked γ ∗ P }}} release l {{{ RET #(); True }}}.
+Lemma release_spec γ l P :
+  {{{ is_lock γ l P ∗ locked γ ∗ P }}} release l {{{ RET #(); True }}}.
 (* SOLUTION *) Proof.
   iIntros "%Φ ((%lo & %ln & -> & #I) & [%o Hexcl] & HP) HΦ".
   wp_lam.
